Use primitive pairs for transformer blocks to make partial evaluation a bit simpler

theories/MaxOfTwoNumbers/Model.v
@@ -1,5 +1,5 @@
 From Coq Require Import Floats Sint63 Uint63 QArith Lia List PArray Morphisms RelationClasses.
-From NeuralNetInterp.Util Require Import Default Pointed PArray List Notations Arith.Classes Arith.Instances Bool Option.
+From NeuralNetInterp.Util Require Import Default Pointed PArray List Notations Arith.Classes Arith.Instances Bool Option PrimitiveProd.
 From NeuralNetInterp.Util Require Nat Wf_Uint63.
 From NeuralNetInterp.Torch Require Import Tensor Einsum Slicing.
 From NeuralNetInterp.TransformerLens Require Import HookedTransformer HookedTransformer.Config HookedTransformer.Module.
@@ -41,7 +41,7 @@ Module Import cfg <: Config.
   Definition blocks_params
     := [(L0_attn_W_Q, L0_attn_W_K, L0_attn_W_V, L0_attn_W_O
           , L0_attn_b_Q, L0_attn_b_K, L0_attn_b_V, L0_attn_b_O
-          , L0_ln1_w, L0_ln1_b)].
+          , L0_ln1_w, L0_ln1_b)%primproj].
 End cfg.
 
 Module Export Model.
