theories/Util/Classes/PrimitiveRelationPairs/Hetero.v
@@ -1,0 +1,81 @@
+(* Adapted from Coq *)
+From Coq Require Import SetoidList Relations Morphisms RelationPairs.
+From NeuralNetInterp.Util.Relations Require Relation_Definitions.Hetero.
+From NeuralNetInterp.Util.Classes Require RelationClasses.Hetero.
+From NeuralNetInterp.Util Require Import PrimitiveProd.
+(*From NeuralNetInterp.Util.Classes Require Morphisms.Hetero.*)
+Import Primitive.
+Import Primitive.Notations.
+
+Local Notation Fst := (@fst _ _).
+Local Notation Snd := (@snd _ _).
+
+Generalizable Variables A B RA RB Ri Ro f.
+
+(** Any function from [A] to [B] allow to obtain a relation over [A]
+    out of a relation over [B]. *)
+
+Definition RelCompFun {A A'} {B B' : Type}(R:Hetero.relation B B')(f:A->B) (f':A'->B') : Hetero.relation A A' :=
+ fun a a' => R (f a) (f' a').
+
+(** Instances on RelCompFun must match syntactically *)
+Global Typeclasses Opaque RelCompFun.
+
+(*
+Infix "@@" := RelCompFun (at level 30, right associativity) : hetero_signature_scope.
+
+Notation "R @@1" := (R @@ Fst)%signature (at level 30) : hetero_signature_scope.
+Notation "R @@2" := (R @@ Snd)%signature (at level 30) : hetero_signature_scope.
+*)
+
+(** We define a product relation over [A*B]: each components should
+    satisfy the corresponding initial relation. *)
+Definition RelProd {A A' B B'} (RA:Hetero.relation A A')(RB:Hetero.relation B B') : Hetero.relation (A*B) (A'*B') :=
+  Hetero.relation_conjunction
+    (@RelCompFun (A * B) (A' * B') A A' RA fst fst)
+    (@RelCompFun (A * B) (A' * B') B B' RB snd snd).
+
+Global Typeclasses Opaque RelProd.
+
+(*Infix "*" := RelProd : hetero_signature_scope.*)
+(*
+Section RelProd_Instances.
+
+  Context {A : Type} {B : Type} (RA : relation A) (RB : relation B).
+
+  Global Instance FstRel_sub :
+    subrelation (RA*RB) (RA @@1).
+  Proof. firstorder. Qed.
+
+  Global Instance SndRel_sub :
+    subrelation (RA*RB) (RB @@2).
+  Proof. firstorder. Qed.
+
+  Global Instance pair_compat :
+    Proper (RA==>RB==> RA*RB) (@pair _ _).
+  Proof. firstorder. Qed.
+
+  Global Instance fst_compat :
+    Proper (RA*RB ==> RA) Fst.
+  Proof.
+    intros (x,y) (x',y') (Hx,Hy); compute in *; auto.
+  Qed.
+
+  Global Instance snd_compat :
+    Proper (RA*RB ==> RB) Snd.
+  Proof.
+    intros (x,y) (x',y') (Hx,Hy); compute in *; auto.
+  Qed.
+
+  Global Instance RelCompFun_compat (f:A->B)
+           `(Proper _ (Ri==>Ri==>Ro) RB) :
+    Proper (Ri@@f==>Ri@@f==>Ro) (RB@@f)%signature.
+  Proof. unfold RelCompFun; firstorder. Qed.
+End RelProd_Instances.
+ *)
+(*
+#[global]
+Hint Unfold RelProd RelCompFun : core.
+#[global]
+Hint Extern 2 (RelProd _ _ _ _) => split : core.
+*)
