theories/Util/Program/PrimitiveBasics/Dependent.v
@@ -1,0 +1,30 @@
+From Coq Require Import Program.Basics Utf8.
+From NeuralNetInterp.Util Require Import PrimitiveProd Program.Basics.Dependent.
+
+Declare Scope primproj_type_function_scope.
+Declare Scope primproj_type_function2_scope.
+Declare Scope primproj_type_function3_scope.
+Declare Scope primproj_type_function4_scope.
+Delimit Scope primproj_type_function_scope with primproj_type_function.
+Delimit Scope primproj_type_function2_scope with primproj_type_function2.
+Delimit Scope primproj_type_function3_scope with primproj_type_function3.
+Delimit Scope primproj_type_function4_scope with primproj_type_function4.
+
+Notation "X * Y" := (fun A : Type => Primitive.prod (X%primproj_type_function%type_function A) (Y%primproj_type_function%type_function A)) : primproj_type_function_scope.
+Notation "X * Y" := (fun A B : Type => Primitive.prod (X%primproj_type_function2%type_function2 A B) (Y%primproj_type_function2%type_function2 A B)) : primproj_type_function2_scope.
+Notation "X * Y" := (fun A B C : Type => Primitive.prod (X%primproj_type_function3%type_function3 A B C) (Y%primproj_type_function3%type_function3 A B C)) : primproj_type_function3_scope.
+Notation "X * Y" := (fun A B C D : Type => Primitive.prod (X%primproj_type_function4%type_function4 A B C D) (Y%primproj_type_function4%type_function4 A B C D)) : primproj_type_function4_scope.
+
+Module Primitive.
+  Export PrimitiveProd.Primitive.
+  Module Notations.
+    Export PrimitiveProd.Primitive.Notations.
+
+    #[export] Set Warnings Append "-notation-overridden".
+    Notation "X * Y" := (fun A : Type => prod (X%type_function A) (Y%type_function A)) : type_function_scope.
+    Notation "X * Y" := (fun A B : Type => prod (X%type_function2 A B) (Y%type_function2 A B)) : type_function2_scope.
+    Notation "X * Y" := (fun A B C : Type => prod (X%type_function3 A B C) (Y%type_function3 A B C)) : type_function3_scope.
+    Notation "X * Y" := (fun A B C D : Type => prod (X%type_function4 A B C D) (Y%type_function4 A B C D)) : type_function4_scope.
+    #[export] Set Warnings Append "notation-overridden".
+  End Notations.
+End Primitive.
